crdt_examples.thy
@@ -289,4 +289,6 @@ definition crdtSpec :: "(structOp, val) crdtSpec" where
 text_raw \<open>}%EndSnippet\<close>
 
 
+
+
 end
